wip: poly1305

code/experimental/poly1305/Hacl.Impl.Poly1305.Field32.fst
@@ -13,6 +13,8 @@ include Hacl.Spec.Poly1305.Field32
 
 module ST = FStar.HyperStack.ST
 module P = NatPrime
+module LSeq = Lib.Sequence
+module BSeq = Lib.ByteSequence
 
 let felem = lbuffer uint32 5ul
 let felem_wide = lbuffer uint64 5ul
@@ -73,6 +75,16 @@ let as_felem (h:mem) (f:felem) : GTot felem5 =
   (s0, s1, s2, s3, s4)
 
 noextract
+let acc_inv_t (h:mem) (acc:felem) : GTot Type0 =
+  let acc = as_felem h acc in
+  acc_inv_t acc
+
+noextract
+let precomp_r5 (h:mem) (r:felem{felem_fits h r (1, 1, 1, 1, 1)}) : GTot felem5 =
+  let r = as_felem h r in
+  precomp_r5 r
+
+noextract
 val fevalh: h:mem -> f:felem -> GTot P.felem
 let fevalh h f = (as_nat h f) % P.prime
 
@@ -85,18 +97,9 @@ val create_felem: unit
   -> StackInline felem
     (requires fun h -> True)
     (ensures  fun h0 b h1 ->
-      stack_allocated b h0 h1 (Lib.Sequence.create 5 (u32 0)) /\
+      stack_allocated b h0 h1 (LSeq.create 5 (u32 0)) /\
       as_nat h1 b == 0)
 let create_felem () = create 5ul (u32 0)
-
-inline_for_extraction
-val create_wide: unit
-  -> StackInline felem_wide
-    (requires fun h -> True)
-    (ensures  fun h0 b h1 ->
-      stack_allocated b h0 h1 (Lib.Sequence.create 5 (u64 0)) /\
-      wide_as_nat h1 b == 0)
-let create_wide () = create 5ul (u64 0)
 
 inline_for_extraction
 val load_felem:
@@ -108,7 +111,7 @@ val load_felem:
     (ensures  fun h0 _ h1 ->
       modifies (loc f) h0 h1 /\
       felem_fits h1 f (1, 1, 1, 1, 1) /\
-      fevalh h1 f == v hi * pow2 64 + v lo)
+      as_nat h1 f == v hi * pow2 64 + v lo)
 let load_felem f lo hi =
   f.(0ul) <- (to_u32 lo) &. mask26;
   f.(1ul) <- (to_u32 (lo >>. 26ul)) &. mask26;
@@ -117,13 +120,49 @@ let load_felem f lo hi =
   f.(4ul) <- to_u32 (hi >>. 40ul); admit()
 
 inline_for_extraction
+val load_felem_le:
+    f:felem
+  -> b:lbuffer uint8 16ul
+  -> Stack unit
+    (requires fun h -> live h f /\ live h b)
+    (ensures  fun h0 _ h1 ->
+      modifies (loc f) h0 h1 /\
+      as_nat h1 f == BSeq.nat_from_bytes_le (as_seq h0 b))
+let load_felem_le f b =
+  let lo = uint_from_bytes_le (sub b 0ul 8ul) in
+  let hi = uint_from_bytes_le (sub b 8ul 8ul) in
+  load_felem f lo hi; admit()
+
+(*
+    let h0 = load32_le (sub b (size 0) (size 4)) in
+    let h1 = load32_le (sub b (size 3) (size 4)) in
+    let h2 = load32_le (sub b (size 6) (size 4)) in
+    let h3 = load32_le (sub b (size 9) (size 4)) in
+    let h4 = load32_le (sub b (size 12) (size 4)) in
+    f.(size 0) <- h0 &. mask26;
+    f.(size 1) <- (h1 >>. u32 2) &. mask26;
+    f.(size 2) <- (h2 >>. u32 4) &. mask26;
+    f.(size 3) <- (h3 >>. u32 6) &. mask26;
+    f.(size 4) <- (h4 >>. u32 8) &. mask26
+*)
+
+inline_for_extraction
+val load_felems_le:
+    f:felem
+  -> b:lbuffer uint8 16ul
+  -> Stack unit
+    (requires fun h -> live h f /\ live h b)
+    (ensures  fun h0 _ h1 -> modifies (loc f) h0 h1)
+let load_felems_le f b = load_felem_le f b
+
+inline_for_extraction
 val store_felem:
     f:felem
   -> Stack (uint64 & uint64)
     (requires fun h ->
-      live h f /\ felem_fits h f (1, 1, 1, 1, 1))
+      live h f /\ felem_fits h f (1, 1, 1, 1, 3))
     (ensures  fun h0 (lo, hi) h1 ->
-      h0 == h1 /\ v hi * pow2 64 + v lo == fevalh h0 f)
+      h0 == h1 /\ v hi * pow2 64 + v lo == (as_nat h0 f) % pow2 128)
 let store_felem f =
   let f0 = to_u64 f.(0ul) |. ((to_u64 f.(1ul)) <<. 26ul) |. ((to_u64 f.(2ul)) <<. 52ul) in
   let f1 = ((to_u64 f.(2ul)) >>. 12ul) |. ((to_u64 f.(3ul)) <<. 14ul) |. ((to_u64 f.(4ul)) <<. 40ul) in
@@ -131,22 +170,41 @@ let store_felem f =
   (f0, f1)
 
 inline_for_extraction
+val store_felem_le:
+    b:lbuffer uint8 16ul
+  -> f:felem
+  -> Stack unit
+    (requires fun h ->
+      live h f /\ live h b /\ felem_fits h f (1, 1, 1, 1, 3))
+    (ensures  fun h0 _ h1 ->
+      modifies (loc f |+| loc b) h0 h1 /\
+      as_seq h1 b == BSeq.nat_to_bytes_le 16 ((as_nat h0 f) % pow2 128))
+let store_felem_le b f =
+  let (f0, f1) = store_felem f in
+  uint_to_bytes_le (sub b 0ul 8ul) f0;
+  uint_to_bytes_le (sub b 8ul 8ul) f1; admit()
+
+inline_for_extraction
 val set_bit:
     f:felem
   -> i:size_t{size_v i < 130}
   -> Stack unit
-    (requires fun h -> live h f)
-    (ensures  fun h0 _ h1 -> modifies (loc f) h0 h1)
-let set_bit f i =
+    (requires fun h -> live h f /\ as_nat h f < pow2 (v i))
+    (ensures  fun h0 _ h1 ->
+      modifies (loc f) h0 h1 /\
+      as_nat h1 f == as_nat h0 f + pow2 (v i))
+let set_bit f i = admit();
   f.(i /. 26ul) <- f.(i /. 26ul) |. (u32 1 <<. (i %. 26ul))
 
 inline_for_extraction
 val set_bit128:
     f:felem
   -> Stack unit
-    (requires fun h -> live h f)
-    (ensures  fun h0 _ h1 -> modifies (loc f) h0 h1)
-let set_bit128 f =
+    (requires fun h -> live h f /\ as_nat h f < pow2 128)
+    (ensures  fun h0 _ h1 ->
+      modifies (loc f) h0 h1 /\
+      as_nat h1 f == as_nat h0 f + pow2 128)
+let set_bit128 f = admit();
   f.(4ul) <- f.(4ul) |. u32 0x1000000
 
 inline_for_extraction
@@ -183,6 +241,28 @@ let copy_felem f1 f2 =
   f1.(3ul) <- f23;
   f1.(4ul) <- f24
 
+inline_for_extraction
+val reduce_felem:
+    f:felem
+  -> Stack unit
+    (requires fun h ->
+      live h f /\ acc_inv_t h f)
+    (ensures  fun h0 _ h1 ->
+      modifies (loc f) h0 h1 /\
+      as_nat h1 f == fevalh h0 f)
+let reduce_felem f =
+  let f0 = f.(0ul) in
+  let f1 = f.(1ul) in
+  let f2 = f.(2ul) in
+  let f3 = f.(3ul) in
+  let f4 = f.(4ul) in
+  let (o0, o1, o2, o3, o4) = reduce_felem5 (f0, f1, f2, f3, f4) in
+  f.(0ul) <- o0;
+  f.(1ul) <- o1;
+  f.(2ul) <- o2;
+  f.(3ul) <- o3;
+  f.(4ul) <- o4
+
 #set-options "--max_fuel 0"
 
 inline_for_extraction
@@ -197,7 +277,8 @@ val load_precompute_r:
      (let r = gsub p 0ul 5ul in
       let r5 = gsub p 5ul 5ul in
       felem_fits h1 r (1, 1, 1, 1, 1) /\
-      as_felem h1 r5 == precomp_r5 (as_felem h1 r)))
+      as_nat h1 r == v r1 * pow2 64 + v r0 /\
+      as_felem h1 r5 == precomp_r5 h1 r))
 let load_precompute_r p r0 r1 =
   let r = sub p 0ul 5ul in
   let r5 = sub p 5ul 5ul in
@@ -216,58 +297,6 @@ let load_precompute_r p r0 r1 =
 
 #reset-options "--z3rlimit 100 --max_fuel 1"
 
-inline_for_extraction
-val fadd_:
-    #m1:scale32_5
-  -> #m2:scale32_5
-  -> out:felem
-  -> f1:felem
-  -> f2:felem
-  -> Stack unit
-    (requires fun h ->
-      live h f1 /\ live h f2 /\ live h out /\
-      felem_fits h f1 m1 /\ felem_fits h f2 m2 /\ (m1 +* m2) <=* s32x5 64)
-    (ensures  fun h0 _ h1 ->
-      modifies (loc out) h0 h1 /\
-      fevalh h1 out == P.fadd (fevalh h0 f1) (fevalh h0 f2))
-let fadd_ #m1 #m2 out f1 f2 =
-  let h0 = ST.get () in
-  let f10 = f1.(0ul) in
-  let f11 = f1.(1ul) in
-  let f12 = f1.(2ul) in
-  let f13 = f1.(3ul) in
-  let f14 = f1.(4ul) in
-  let f20 = f2.(0ul) in
-  let f21 = f2.(1ul) in
-  let f22 = f2.(2ul) in
-  let f23 = f2.(3ul) in
-  let f24 = f2.(4ul) in
-  out.(0ul) <- f10 +! f20;
-  out.(1ul) <- f11 +! f21;
-  out.(2ul) <- f12 +! f22;
-  out.(3ul) <- f13 +! f23;
-  out.(4ul) <- f14 +! f24;
-  let h1 = ST.get () in
-  assert (as_nat h1 out == as_nat h0 f1 + as_nat h0 f2);
-  FStar.Math.Lemmas.lemma_mod_plus_distr_l
-    (as_nat h0 f1) (as_nat h0 f2) P.prime;
-  FStar.Math.Lemmas.lemma_mod_plus_distr_r
-    (as_nat h0 f1 % P.prime) (as_nat h0 f2) P.prime
-
-[@CInline]
-val fadd:
-    out:felem
-  -> f1:felem
-  -> f2:felem
-  -> Stack unit
-    (requires fun h ->
-      live h f1 /\ live h f2 /\ live h out /\
-      felem_fits h f1 (s32x5 32) /\ felem_fits h f2 (s32x5 32))
-    (ensures  fun h0 _ h1 ->
-      modifies (loc out) h0 h1 /\
-      fevalh h1 out == P.fadd (fevalh h0 f1) (fevalh h0 f2))
-let fadd out f1 f2 = fadd_ #(s32x5 32) #(s32x5 32) out f1 f2
-
 //inline_for_extraction
 [@CInline]
 val fmul_r:
@@ -282,10 +311,10 @@ val fmul_r:
       let r5 = gsub p 5ul 5ul in
       felem_fits h r (1, 1, 1, 1, 1) /\
       felem_fits h r5 (5, 5, 5, 5, 5) /\
-      as_felem h r5 == precomp_r5 (as_felem h r)))
+      as_felem h r5 == precomp_r5 h r))
     (ensures fun h0 _ h1 ->
       modifies (loc out) h0 h1 /\
-      acc_inv_t (as_felem h1 out) /\
+      acc_inv_t h1 out /\
      (let r = gsub p 0ul 5ul in
       let r5 = gsub p 5ul 5ul in
       fevalh h1 out == P.fmul (fevalh h0 f1) (fevalh h0 r)))
@@ -334,10 +363,10 @@ val fadd_mul_r:
       let r5 = gsub p 5ul 5ul in
       felem_fits h r (1, 1, 1, 1, 1) /\
       felem_fits h r5 (5, 5, 5, 5, 5) /\
-      as_felem h r5 == precomp_r5 (as_felem h r)))
+      as_felem h r5 == precomp_r5 h r))
     (ensures  fun h0 _ h1 ->
       modifies (loc out) h0 h1 /\
-      acc_inv_t (as_felem h1 out) /\
+      acc_inv_t h1 out /\
      (let r = gsub p 0ul 5ul in
       let r5 = gsub p 5ul 5ul in
       fevalh h1 out == P.fmul (P.fadd (fevalh h0 out) (fevalh h0 f1)) (fevalh h0 r)))
@@ -390,10 +419,10 @@ val fmul_rn:
       let r5 = gsub p 5ul 5ul in
       felem_fits h r (1, 1, 1, 1, 1) /\
       felem_fits h r5 (5, 5, 5, 5, 5) /\
-      as_felem h r5 == precomp_r5 (as_felem h r)))
+      as_felem h r5 == precomp_r5 h r))
     (ensures  fun h0 _ h1 ->
       modifies (loc out) h0 h1 /\
-      acc_inv_t (as_felem h1 out) /\
+      acc_inv_t h1 out /\
      (let r = gsub p 0ul 5ul in
       let r5 = gsub p 5ul 5ul in
       fevalh h1 out == P.fmul (fevalh h0 f1) (fevalh h0 r)))
@@ -412,108 +441,110 @@ val fmul_rn_normalize:
       let r5 = gsub p 5ul 5ul in
       felem_fits h r (1, 1, 1, 1, 1) /\
       felem_fits h r5 (5, 5, 5, 5, 5) /\
-      as_felem h r5 == precomp_r5 (as_felem h r)))
+      as_felem h r5 == precomp_r5 h r))
     (ensures  fun h0 _ h1 ->
       modifies (loc out) h0 h1 /\
-      acc_inv_t (as_felem h1 out) /\
+      acc_inv_t h1 out /\
      (let r = gsub p 0ul 5ul in
       let r5 = gsub p 5ul 5ul in
       fevalh h1 out == P.fmul (fevalh h0 out) (fevalh h0 r)))
 let fmul_rn_normalize out p =
   fmul_r out out p
 
-inline_for_extraction
-val reduce_felem:
-    f:felem
+[@CInline]
+val fadd:
+    out:felem
+  -> f1:felem
+  -> f2:felem
   -> Stack unit
     (requires fun h ->
-      live h f /\ acc_inv_t (as_felem h f))
+      live h f1 /\ live h f2 /\ live h out /\
+      felem_fits h f1 (1, 2, 1, 1, 1) /\
+      felem_fits h f2 (1, 1, 1, 1, 1))
     (ensures  fun h0 _ h1 ->
-      modifies (loc f) h0 h1 /\
-      as_nat h1 f == fevalh h0 f)
-let reduce_felem f =
-  let f0 = f.(0ul) in
-  let f1 = f.(1ul) in
-  let f2 = f.(2ul) in
-  let f3 = f.(3ul) in
-  let f4 = f.(4ul) in
-  let (o0, o1, o2, o3, o4) = reduce_felem5 (f0, f1, f2, f3, f4) in
-  f.(0ul) <- o0;
-  f.(1ul) <- o1;
-  f.(2ul) <- o2;
-  f.(3ul) <- o3;
-  f.(4ul) <- o4
+      modifies (loc out) h0 h1 /\
+      felem_fits h1 out (2, 3, 2, 2, 2) /\
+      fevalh h1 out == P.fadd (fevalh h0 f1) (fevalh h0 f2))
+let fadd out f1 f2 =
+  let h0 = ST.get () in
+  let f10 = f1.(0ul) in
+  let f11 = f1.(1ul) in
+  let f12 = f1.(2ul) in
+  let f13 = f1.(3ul) in
+  let f14 = f1.(4ul) in
+  let f20 = f2.(0ul) in
+  let f21 = f2.(1ul) in
+  let f22 = f2.(2ul) in
+  let f23 = f2.(3ul) in
+  let f24 = f2.(4ul) in
+  out.(0ul) <- f10 +! f20;
+  out.(1ul) <- f11 +! f21;
+  out.(2ul) <- f12 +! f22;
+  out.(3ul) <- f13 +! f23;
+  out.(4ul) <- f14 +! f24;
+  let h1 = ST.get () in
+  assert (as_nat h1 out == as_nat h0 f1 + as_nat h0 f2);
+  FStar.Math.Lemmas.lemma_mod_plus_distr_l
+    (as_nat h0 f1) (as_nat h0 f2) P.prime;
+  FStar.Math.Lemmas.lemma_mod_plus_distr_r
+    (as_nat h0 f1 % P.prime) (as_nat h0 f2) P.prime
 
-inline_for_extraction
-val load_felem_le:
-    f:felem
-  -> b:lbuffer uint8 16ul
+val lemma_fadd128:
+    f:felem5 -> tmp:felem5
+  -> c0:uint32 -> c1:uint32 -> c2:uint32 -> c3:uint32
+  -> Lemma
+    (requires
+      (let (tmp0, tmp1, tmp2, tmp3, tmp4) = tmp in
+      as_nat5 f == v tmp0 + v c0 * pow2 26 + (v tmp1 + v c1 * pow2 26 - v c0) * pow26 +
+      (v tmp2 + v c2 * pow2 26 - v c1) * pow26 * pow26 + (v tmp3 + v c3 * pow2 26 - v c2) * pow26 * pow26 * pow26 +
+      (v tmp4 - v c3) * pow26 * pow26 * pow26 * pow26))
+    (ensures as_nat5 f == as_nat5 tmp)
+let lemma_fadd128 f tmp c0 c1 c2 c3 = ()
+
+val fadd_carry:
+    out:felem
+  -> f1:felem
+  -> f2:felem
   -> Stack unit
-    (requires fun h -> live h f /\ live h b)
-    (ensures  fun h0 _ h1 -> modifies (loc f) h0 h1)
-let load_felem_le f b =
-  let lo = uint_from_bytes_le (sub b 0ul 8ul) in
-  let hi = uint_from_bytes_le (sub b 8ul 8ul) in
-  load_felem f lo hi
-
-(*
-    let h0 = load32_le (sub b (size 0) (size 4)) in
-    let h1 = load32_le (sub b (size 3) (size 4)) in
-    let h2 = load32_le (sub b (size 6) (size 4)) in
-    let h3 = load32_le (sub b (size 9) (size 4)) in
-    let h4 = load32_le (sub b (size 12) (size 4)) in
-    f.(size 0) <- h0 &. mask26;
-    f.(size 1) <- (h1 >>. u32 2) &. mask26;
-    f.(size 2) <- (h2 >>. u32 4) &. mask26;
-    f.(size 3) <- (h3 >>. u32 6) &. mask26;
-    f.(size 4) <- (h4 >>. u32 8) &. mask26
-*)
-
-inline_for_extraction
-val load_felems_le:
-    f:felem
-  -> b:lbuffer uint8 16ul
-  -> Stack unit
-    (requires fun h -> live h f /\ live h b)
-    (ensures  fun h0 _ h1 -> modifies (loc f) h0 h1)
-let load_felems_le f b = load_felem_le f b
-
-inline_for_extraction
-val carry_felem:
-    f:felem
-  -> Stack unit
-    (requires fun h -> live h f /\ acc_inv_t (as_felem h f))
+    (requires fun h ->
+      live h f1 /\ live h f2 /\ live h out /\
+      felem_fits h f1 (1, 1, 1, 1, 1) /\
+      felem_fits h f2 (1, 1, 1, 1, 1))
     (ensures  fun h0 _ h1 ->
-      modifies (loc f) h0 h1 /\
-      felem_fits h1 f (1,1,1,1,1) /\
-      fevalh h1 f == fevalh h0 f)
-let carry_felem f =
-  let f0 = f.(0ul) in
-  let f1 = f.(1ul) in
-  let f2 = f.(2ul) in
-  let f3 = f.(3ul) in
-  let f4 = f.(4ul) in
+      modifies (loc out) h0 h1 /\
+      as_nat h1 out == as_nat h0 f1 + as_nat h0 f2 /\
+      felem_fits h1 out (1, 1, 1, 1, 3))
+let fadd_carry out f1 f2 =
+  let f10 = f1.(0ul) in
+  let f11 = f1.(1ul) in
+  let f12 = f1.(2ul) in
+  let f13 = f1.(3ul) in
+  let f14 = f1.(4ul) in
+  let f20 = f2.(0ul) in
+  let f21 = f2.(1ul) in
+  let f22 = f2.(2ul) in
+  let f23 = f2.(3ul) in
+  let f24 = f2.(4ul) in
+  [@inline_let]
+  let f0 = f10 +! f20 in
+  [@inline_let]
+  let f1 = f11 +! f21 in
+  [@inline_let]
+  let f2 = f12 +! f22 in
+  [@inline_let]
+  let f3 = f13 +! f23 in
+  [@inline_let]
+  let f4 = f14 +! f24 in
+  assert (felem_fits5 (f0, f1, f2, f3, f4) (2, 2, 2, 2, 2));
   let tmp0, c0 = carry26 f0 (u32 0) in
   let tmp1, c1 = carry26 f1 c0 in
   let tmp2, c2 = carry26 f2 c1 in
   let tmp3, c3 = carry26 f3 c2 in
-  let tmp4 = f4 +. c3 in
-  admit();
-  f.(0ul) <- tmp0;
-  f.(1ul) <- tmp1;
-  f.(2ul) <- tmp2;
-  f.(3ul) <- tmp3;
-  f.(4ul) <- tmp4
-
-inline_for_extraction
-val store_felem_le:
-    b:lbuffer uint8 16ul
-  -> f:felem
-  -> Stack unit
-    (requires fun h -> live h f /\ live h b /\ acc_inv_t (as_felem h f))
-    (ensures  fun h0 _ h1 -> modifies (loc f |+| loc b) h0 h1)
-let store_felem_le b f =
-  carry_felem f;
-  let (f0, f1) = store_felem f in
-  uint_to_bytes_le (sub b 0ul 8ul) f0;
-  uint_to_bytes_le (sub b 8ul 8ul) f1
+  let tmp4 = f4 +! c3 in
+  lemma_fadd128 (f0, f1, f2, f3, f4) (tmp0, tmp1, tmp2, tmp3, tmp4) c0 c1 c2 c3;
+  assert (felem_fits5 (tmp0, tmp1, tmp2, tmp3, tmp4) (1, 1, 1, 1, 3));
+  out.(0ul) <- tmp0;
+  out.(1ul) <- tmp1;
+  out.(2ul) <- tmp2;
+  out.(3ul) <- tmp3;
+  out.(4ul) <- tmp4
