code/experimental/poly1305/Hacl.Impl.Poly1305.Fields.fst
@@ -2,6 +2,7 @@ module Hacl.Impl.Poly1305.Fields
 
 open FStar.HyperStack
 open FStar.HyperStack.All
+open FStar.Mul
 
 open Lib.IntTypes
 open Lib.Buffer
@@ -12,6 +13,8 @@ open Lib.Vec256
 
 module ST = FStar.HyperStack.ST
 module P = NatPrime
+module LSeq = Lib.Sequence
+module BSeq = Lib.ByteSequence
 
 module F32 = Hacl.Impl.Poly1305.Field32
 module F64 = Hacl.Impl.Poly1305.Field64
@@ -108,7 +111,7 @@ val create_felem:
   -> StackInline (felem s)
     (requires fun h -> True)
     (ensures  fun h0 f h1 ->
-      stack_allocated f h0 h1 (Lib.Sequence.create (v (nlimb s)) (limb_zero s)) /\
+      stack_allocated f h0 h1 (LSeq.create (v (nlimb s)) (limb_zero s)) /\
       as_nat h1 f == 0)
 let create_felem s =
   match s with
@@ -124,13 +127,15 @@ val load_felem_le:
   -> b:lbuffer uint8 16ul
   -> Stack unit
     (requires fun h -> live h f /\ live h b)
-    (ensures  fun h0 _ h1 -> modifies (loc f) h0 h1)
+    (ensures  fun h0 _ h1 ->
+      modifies (loc f) h0 h1 /\
+      as_nat h1 f == BSeq.nat_from_bytes_le (as_seq h0 b))
 let load_felem_le #s f b =
   match s with
   | M32 -> F32.load_felem_le f b
-  | M64 -> F64.load_felem_le f b
-  | M128 -> F128.load_felem_le f b
-  | M256 -> F256.load_felem_le f b
+  | M64 -> admit(); F64.load_felem_le f b
+  | M128 -> admit(); F128.load_felem_le f b
+  | M256 -> admit(); F256.load_felem_le f b
 
 inline_for_extraction
 val load_felems_le:
@@ -147,20 +152,30 @@ let load_felems_le #s f b =
   | M128 -> F128.load_felems_le f b
   | M256 -> F256.load_felems_le f b
 
+val store_felem_le_pre: #s:field_spec -> h:mem -> f:felem s -> Type0
+let store_felem_le_pre #s h f =
+  match s with
+  | M32 -> F32.felem_fits h f (1, 1, 1, 1, 3)
+  | M64 -> True
+  | M128 -> True
+  | M256 -> True
+
 inline_for_extraction
 val store_felem_le:
     #s:field_spec
   -> b:lbuffer uint8 16ul
   -> f:felem s
   -> Stack unit
-    (requires fun h -> live h f /\ live h b)
-    (ensures  fun h0 _ h1 -> modifies (loc b |+| loc f) h0 h1)
+    (requires fun h -> live h f /\ live h b /\ store_felem_le_pre h f)
+    (ensures  fun h0 _ h1 ->
+      modifies (loc b |+| loc f) h0 h1 /\
+      as_seq h1 b == BSeq.nat_to_bytes_le 16 ((as_nat h0 f) % pow2 128))
 let store_felem_le #s b f =
   match s with
-  | M32 -> admit(); F32.store_felem_le b f
-  | M64 -> F64.store_felem_le b f
-  | M128 -> F128.store_felem_le b f
-  | M256 -> F256.store_felem_le b f
+  | M32 -> F32.store_felem_le b f
+  | M64 -> admit(); F64.store_felem_le b f
+  | M128 -> admit(); F128.store_felem_le b f
+  | M256 -> admit(); F256.store_felem_le b f
 
 inline_for_extraction
 val set_bit:
@@ -168,28 +183,32 @@ val set_bit:
   -> f:felem s
   -> i:size_t{size_v i < 130}
   -> Stack unit
-    (requires fun h -> live h f)
-    (ensures  fun h0 _ h1 -> modifies (loc f) h0 h1)
+    (requires fun h -> live h f /\ as_nat h f < pow2 (v i))
+    (ensures  fun h0 _ h1 ->
+      modifies (loc f) h0 h1 /\
+      as_nat h1 f == as_nat h0 f + pow2 (v i))
 let set_bit #s f i =
   match s with
   | M32 -> F32.set_bit f i
-  | M64 -> F64.set_bit f i
-  | M128 -> F128.set_bit f i
-  | M256 -> F256.set_bit f i
+  | M64 -> admit(); F64.set_bit f i
+  | M128 -> admit(); F128.set_bit f i
+  | M256 -> admit(); F256.set_bit f i
 
 inline_for_extraction
 val set_bit128:
     #s:field_spec
   -> f:felem s
   -> Stack unit
-    (requires fun h -> live h f)
-    (ensures  fun h0 _ h1 -> modifies (loc f) h0 h1)
+    (requires fun h -> live h f /\ as_nat h f < pow2 128)
+    (ensures  fun h0 _ h1 ->
+      modifies (loc f) h0 h1 /\
+      as_nat h1 f == as_nat h0 f + pow2 128)
 let set_bit128 #s f =
   match s with
   | M32 -> F32.set_bit128 f
-  | M64 -> F64.set_bit128 f
-  | M128 -> F128.set_bit128 f
-  | M256 -> F256.set_bit128 f
+  | M64 -> admit(); F64.set_bit128 f
+  | M128 -> admit(); F128.set_bit128 f
+  | M256 -> admit(); F256.set_bit128 f
 
 inline_for_extraction
 val set_zero:
@@ -222,19 +241,39 @@ let copy_felem #s f f' =
   | M128 -> admit(); F128.copy_felem f f'
   | M256 -> admit(); F256.copy_felem f f'
 
+val reduce_felem_pre: #s:field_spec -> h:mem -> f:felem s -> Type0
+let reduce_felem_pre #s h f =
+  match s with
+  | M32 -> F32.acc_inv_t h f
+  | M64 -> True
+  | M128 -> True
+  | M256 -> True
+
 inline_for_extraction
 val reduce_felem:
     #s:field_spec
   -> f:felem s
   -> Stack unit
-    (requires fun h -> live h f)
-    (ensures  fun h0 _ h1 -> modifies (loc f) h0 h1)
+    (requires fun h -> live h f /\ reduce_felem_pre h f)
+    (ensures  fun h0 _ h1 ->
+      modifies (loc f) h0 h1 /\
+      as_nat h1 f == feval h0 f)
 let reduce_felem #s f =
   match s with
-  | M32 -> admit(); F32.reduce_felem f
-  | M64 -> F64.reduce_felem f
-  | M128 -> F128.reduce_felem f
-  | M256 -> F256.reduce_felem f
+  | M32 -> F32.reduce_felem f
+  | M64 -> admit(); F64.reduce_felem f
+  | M128 -> admit(); F128.reduce_felem f
+  | M256 -> admit(); F256.reduce_felem f
+
+val load_precompute_r_post: #s:field_spec -> h:mem -> r:felem s -> r5:felem s -> Type0
+let load_precompute_r_post #s h r r5 =
+  match s with
+  | M32 -> F32.felem_fits h r (1, 1, 1, 1, 1) /\
+           F32.felem_fits h r5 (5, 5, 5, 5, 5) /\
+           F32.as_felem h r5 == F32.precomp_r5 h r
+  | M64 -> True
+  | M128 -> True
+  | M256 -> True
 
 inline_for_extraction
 val load_precompute_r:
@@ -244,13 +283,26 @@ val load_precompute_r:
   -> r1:uint64
   -> Stack unit
     (requires fun h -> live h p)
-    (ensures  fun h0 _ h1 -> modifies (loc p) h0 h1)
+    (ensures  fun h0 _ h1 ->
+      modifies (loc p) h0 h1 /\
+     (let r = gsub p 0ul (nlimb s) in
+      let r5 = gsub p (nlimb s) (nlimb s) in
+      load_precompute_r_post h1 r r5 /\
+      as_nat h1 r == v r1 * pow2 64 + v r0))
 let load_precompute_r #s p r0 r1 =
   match s with
-  | M32 -> admit(); F32.load_precompute_r p r0 r1
-  | M64 -> F64.load_precompute_r p r0 r1
-  | M128 -> F128.load_precompute_r p r0 r1
-  | M256 -> F256.load_precompute_r p r0 r1
+  | M32 -> F32.load_precompute_r p r0 r1
+  | M64 -> admit(); F64.load_precompute_r p r0 r1
+  | M128 -> admit(); F128.load_precompute_r p r0 r1
+  | M256 -> admit(); F256.load_precompute_r p r0 r1
+
+val fmul_r_pre: #s:field_spec -> h:mem -> f1:felem s -> r:felem s -> r5:felem s -> Type0
+let fmul_r_pre #s h f1 r r5 =
+  match s with
+  | M32 -> F32.felem_fits h f1 (2, 3, 2, 2, 2) /\ load_precompute_r_post h r r5
+  | M64 -> True
+  | M128 -> True
+  | M256 -> True
 
 inline_for_extraction
 val fmul_r:
@@ -259,14 +311,33 @@ val fmul_r:
   -> f1:felem s
   -> precomp:precomp_r s
   -> Stack unit
-    (requires fun h -> live h out /\ live h f1 /\ live h precomp)
-    (ensures  fun h0 _ h1 -> modifies (loc out) h0 h1)
+    (requires fun h ->
+      live h out /\ live h f1 /\ live h precomp /\
+     (let r = gsub precomp 0ul (nlimb s) in
+      let r5 = gsub precomp (nlimb s) (nlimb s) in
+      fmul_r_pre h f1 r r5))
+    (ensures  fun h0 _ h1 ->
+      modifies (loc out) h0 h1 /\
+      reduce_felem_pre h1 out /\
+     (let r = gsub precomp 0ul (nlimb s) in
+      let r5 = gsub precomp (nlimb s) (nlimb s) in
+      feval h1 out == P.fmul (feval h0 f1) (feval h0 r)))
 let fmul_r #s out f1 precomp =
   match s with
-  | M32 -> admit(); F32.fmul_r out f1 precomp
-  | M64 -> F64.fmul_r out f1 precomp
-  | M128 -> F128.fmul_r out f1 precomp
-  | M256 -> F256.fmul_r out f1 precomp
+  | M32 -> F32.fmul_r out f1 precomp
+  | M64 -> admit(); F64.fmul_r out f1 precomp
+  | M128 -> admit(); F128.fmul_r out f1 precomp
+  | M256 -> admit(); F256.fmul_r out f1 precomp
+
+val fadd_mul_r_pre: #s:field_spec -> h:mem -> out:felem s -> f1:felem s -> r:felem s -> r5:felem s -> Type0
+let fadd_mul_r_pre #s h out f1 r r5 =
+  match s with
+  | M32 -> F32.felem_fits h f1 (1, 1, 1, 1, 1) /\
+           F32.felem_fits h out (1, 2, 1, 1, 1) /\
+           load_precompute_r_post h r r5
+  | M64 -> True
+  | M128 -> True
+  | M256 -> True
 
 inline_for_extraction
 val fadd_mul_r:
@@ -275,14 +346,23 @@ val fadd_mul_r:
   -> f1:felem s
   -> precomp:precomp_r s
   -> Stack unit
-    (requires fun h -> live h out /\ live h f1 /\ live h precomp)
-    (ensures  fun h0 _ h1 -> modifies (loc out) h0 h1)
+    (requires fun h ->
+      live h out /\ live h f1 /\ live h precomp /\
+     (let r = gsub precomp 0ul (nlimb s) in
+      let r5 = gsub precomp (nlimb s) (nlimb s) in
+      fadd_mul_r_pre h out f1 r r5))
+    (ensures  fun h0 _ h1 ->
+      modifies (loc out) h0 h1 /\
+      reduce_felem_pre h1 out /\
+     (let r = gsub precomp 0ul (nlimb s) in
+      let r5 = gsub precomp (nlimb s) (nlimb s) in
+      feval h1 out == P.fmul (P.fadd (feval h0 out) (feval h0 f1)) (feval h0 r)))
 let fadd_mul_r #s out f1 precomp =
   match s with
-  | M32 -> admit(); F32.fadd_mul_r out f1 precomp
-  | M64 -> F64.fadd_mul_r out f1 precomp
-  | M128 -> F128.fadd_mul_r out f1 precomp
-  | M256 -> F256.fadd_mul_r out f1 precomp
+  | M32 -> F32.fadd_mul_r out f1 precomp
+  | M64 -> admit(); F64.fadd_mul_r out f1 precomp
+  | M128 -> admit(); F128.fadd_mul_r out f1 precomp
+  | M256 -> admit(); F256.fadd_mul_r out f1 precomp
 
 inline_for_extraction
 val fmul_rn:
@@ -315,6 +395,23 @@ let fmul_rn_normalize #s out precomp =
   | M128 -> F128.fmul_rn_normalize out precomp
   | M256 -> F256.fmul_rn_normalize out precomp
 
+val fadd_pre: #s:field_spec -> h:mem -> f1:felem s -> f2:felem s -> Type0
+let fadd_pre #s h f1 f2 =
+  match s with
+  | M32 -> F32.felem_fits h f1 (1, 2, 1, 1, 1) /\
+           F32.felem_fits h f2 (1, 1, 1, 1, 1)
+  | M64 -> True
+  | M128 -> True
+  | M256 -> True
+
+val fadd_post: #s:field_spec -> h:mem -> out:felem s -> Type0
+let fadd_post #s h out =
+  match s with
+  | M32 -> F32.felem_fits h out (2, 3, 2, 2, 2)
+  | M64 -> True
+  | M128 -> True
+  | M256 -> True
+
 inline_for_extraction
 val fadd:
     #s:field_spec
@@ -322,11 +419,50 @@ val fadd:
   -> f1:felem s
   -> f2:felem s
   -> Stack unit
-    (requires fun h -> live h out /\ live h f1 /\ live h f2)
-    (ensures  fun h0 _ h1 -> modifies (loc out) h0 h1)
+    (requires fun h ->
+      live h out /\ live h f1 /\ live h f2 /\ fadd_pre h f1 f2)
+    (ensures  fun h0 _ h1 ->
+      modifies (loc out) h0 h1 /\ fadd_post h1 out /\
+      feval h1 out == P.fadd (feval h0 f1) (feval h0 f2))
 let fadd #s out f1 f2=
   match s with
-  | M32 -> admit(); F32.fadd out f1 f2
+  | M32 -> F32.fadd out f1 f2
   | M64 -> admit(); F64.fadd out f1 f2
-  | M128 -> F128.fadd out f1 f2
-  | M256 -> F256.fadd out f1 f2
+  | M128 -> admit(); F128.fadd out f1 f2
+  | M256 -> admit(); F256.fadd out f1 f2
+
+val fadd_carry_pre: #s:field_spec -> h:mem -> f1:felem s -> f2:felem s -> Type0
+let fadd_carry_pre #s h f1 f2 =
+  match s with
+  | M32 -> F32.felem_fits h f1 (1, 1, 1, 1, 1) /\
+           F32.felem_fits h f2 (1, 1, 1, 1, 1)
+  | M64 -> True
+  | M128 -> True
+  | M256 -> True
+
+val fadd_carry_post: #s:field_spec -> h:mem -> out:felem s -> Type0
+let fadd_carry_post #s h out =
+  match s with
+  | M32 -> F32.felem_fits h out (1, 1, 1, 1, 3)
+  | M64 -> True
+  | M128 -> True
+  | M256 -> True
+
+inline_for_extraction
+val fadd_carry:
+    #s:field_spec
+  -> out:felem s
+  -> f1:felem s
+  -> f2:felem s
+  -> Stack unit
+    (requires fun h ->
+      live h out /\ live h f1 /\ live h f2 /\ fadd_carry_pre h f1 f2)
+    (ensures  fun h0 _ h1 ->
+      modifies (loc out) h0 h1 /\ fadd_carry_post h1 out /\
+      as_nat h1 out == as_nat h0 f1 + as_nat h0 f2)
+let fadd_carry #s out f1 f2=
+  match s with
+  | M32 -> F32.fadd_carry out f1 f2
+  | M64 -> admit(); F64.fadd out f1 f2
+  | M128 -> admit(); F128.fadd out f1 f2
+  | M256 -> admit(); F256.fadd out f1 f2
